Type annotations on expressions: fully abstracted operators' semantics. Still, the layer doesn't work due to module type instanciation issue.

Correctness/IsPresent.v
@@ -18,7 +18,7 @@ to tie the result of [Control ck] with the dataflow semantics of
 Assumption: the base clock is [true] *)
 
 Module Type ISPRESENT
-       (Op : OPERATORS)
+       (Import Op : OPERATORS)
        (Import SynDF : Rustre.Dataflow.Syntax.SYNTAX Op)
        (Import SynMP : Rustre.Minimp.Syntax.SYNTAX Op)
        (Import SemMP : Rustre.Minimp.Semantics.SEMANTICS Op SynMP)
@@ -28,30 +28,30 @@ Module Type ISPRESENT
   : clock -> Prop :=
   | IsCbase: Is_present_in mems heap stack Cbase
   | IsCon:
-      forall ck c v,
+      forall ck c ty v,
         Is_present_in mems heap stack ck
-        -> exp_eval heap stack (tovar mems c) (Op.Vbool v)
-        -> Is_present_in mems heap stack (Con ck c v).
+        -> exp_eval heap stack (tovar mems (c, ty)) (Vbool v)
+        -> Is_present_in mems heap stack (Con ck c ty v).
 
   Inductive Is_absent_in (mems: PS.t) heap stack: clock -> Prop :=
   | IsAbs1:
-      forall ck c v,
+      forall ck c ty v,
         Is_absent_in mems heap stack ck
-        -> Is_absent_in mems heap stack (Con ck c v)
+        -> Is_absent_in mems heap stack (Con ck c ty v)
   | IsAbs2:
-      forall ck c v1 v2,
+      forall ck c ty v1 v2,
         Is_present_in mems heap stack ck
-        -> exp_eval heap stack (tovar mems c) (Op.Vbool v1)
+        -> exp_eval heap stack (tovar mems (c, ty)) (Vbool v1)
         -> v2 <> v1
-        -> Is_absent_in mems heap stack (Con ck c v2).
+        -> Is_absent_in mems heap stack (Con ck c ty v2).
 
 
   (** ** Properties *)
 
   Lemma exp_eval_tovar_Cbool_dec:
     forall menv env mems c v,
-      {exp_eval menv env (tovar mems c) (Op.Vbool v)}
-      + {~exp_eval menv env (tovar mems c) (Op.Vbool v)}.
+      {exp_eval menv env (tovar mems c) (Vbool v)}
+      + {~exp_eval menv env (tovar mems c) (Vbool v)}.
   Proof.
     Ltac no_match := right; inversion_clear 1; try unfold mfind_mem in *;
                      match goal with
@@ -59,7 +59,7 @@ Module Type ISPRESENT
                           H': PM.find _ _ = _ |- _ => rewrite H in H'; discriminate
                      end.
     intros menv env mems c v.
-    unfold tovar.
+    unfold tovar; destruct c as [c ty].
     destruct (PS.mem c mems).
     - case_eq (mfind_mem c menv).
       + intro c0; destruct c0.
@@ -81,21 +81,21 @@ Module Type ISPRESENT
     induction ck.
     - left; constructor.
     - destruct IHck.
-      + destruct (exp_eval_tovar_Cbool_dec menv env mems i b); destruct b;
+      + destruct (exp_eval_tovar_Cbool_dec menv env mems (i, t) b); destruct b;
         (left; constructor; assumption) || right; inversion_clear 1; auto.
       + right; inversion_clear 1; auto.
   Qed.
 
 
   Lemma Is_absent_in_disj:
-    forall mems menv env ck c v,
-      Is_absent_in mems menv env (Con ck c v)
+    forall mems menv env ck c ty v,
+      Is_absent_in mems menv env (Con ck c ty v)
       -> (Is_absent_in mems menv env ck
-         \/ (forall v', exp_eval menv env (tovar mems c) (Op.Vbool v')
+         \/ (forall v', exp_eval menv env (tovar mems (c, ty)) (Vbool v')
                   -> v' <> v)).
   Proof.
     intros until c.
-    inversion_clear 1 as [ | ? ? ? ? Hp Hexp Hneq]; intuition.
+    inversion_clear 1 as [ | ? ? ? ? ? Hp Hexp Hneq]; intuition.
     right; intros v' Hexp'.
     intro HR; rewrite <-HR in *; clear HR.
     apply Hneq.
